src/typechecker/FStar.TypeChecker.Primops.Docs.fsti
@@ -1,0 +1,5 @@
+module FStar.TypeChecker.Primops.Docs
+
+open FStar.TypeChecker.Primops.Base
+
+val doc_ops : list primitive_step
